simplify morphism definition; reprove induction; introduce first notions of (weak) equivalence

execution/theories/ContractMorphisms.v
@@ -18,222 +18,105 @@ From ConCert.Execution Require Import BuildUtils.
 From ConCert.Execution Require Import InterContractCommunication.
 From ConCert.Utils Require Import RecordUpdate.
 
-(* TODO USE `GENERALIZE VARIABLE` SYNTAX TO GET RID OF ALL THE IMPLICIT NOTATION *)
-
-(* some auxiliary functions *)
-Definition curry_3 {A B C D : Type} (f : A * B * C -> D) : A -> B -> C -> D := 
-    (compose curry curry) f.
-Definition curry_4 {A B C D E : Type} (f : A * B * C * D -> E) : A -> B -> C -> D -> E :=
-    curry (curry (curry f)).
-Definition uncurry_3 {A B C D : Type} (f : A -> B -> C -> D) : A * B * C -> D :=
-    (compose uncurry uncurry) f.
-Definition uncurry_4 {A B C D E : Type} (f : A -> B -> C -> D -> E) : A * B * C * D -> E :=
-    uncurry (uncurry (uncurry f)).
-
 Section ContractMorphisms.
 Context { Base : ChainBase }.
 
+Definition result_functor {T T' E E' : Type} : (T -> T') -> (E -> E') -> result T E -> result T' E' :=
+    fun (f_t : T -> T') (f_e : E -> E') (res : result T E) => 
+    match res with | Ok t => Ok (f_t t) | Err e => Err (f_e e) end.
+
 (** First, a definition of a Contract Morphism, which is a function between contracts *)
 Section MorphismDefinition.
-Context `{Serializable Msg}  `{Serializable Setup}  `{Serializable State}  `{Serializable Error}
-    `{Serializable Msg'} `{Serializable Setup'} `{Serializable State'} `{Serializable Error'}.
-
-(** The init component *)
-Record InitCM (C : Contract Setup Msg State Error) (C' : Contract Setup' Msg' State' Error') 
-    := build_init_cm {
-        (* transform inputs/outputs of the init function *)
-        init_inputs : Chain * ContractCallContext * Setup -> 
-            Chain * ContractCallContext * Setup' ;
-        init_outputs : result State Error -> result State' Error' ;
-        (* proof of commutativity *)
-        init_commutes : 
-            forall x : Chain * ContractCallContext * Setup,
-                uncurry_3 (init C') (init_inputs x) = 
-                init_outputs (uncurry_3 (init C) x) ;
-    }.
-
-(** The receive component *)
-Record RecvCM (C : Contract Setup Msg State Error) (C' : Contract Setup' Msg' State' Error') := 
-    build_recv_cm {
-        (* transform inputs/outputs of the receive function *)
-        recv_inputs : Chain * ContractCallContext * State * option Msg -> 
-            Chain * ContractCallContext * State' * option Msg' ;
-        recv_outputs : result (State * list ActionBody) Error -> 
-            result (State' * list ActionBody) Error' ;
-        (* proof of commutativity *)
-        recv_commutes : 
-            forall (x : Chain * ContractCallContext * State * option Msg), 
-                uncurry_4 (receive C') (recv_inputs x) = 
-                recv_outputs (uncurry_4 (receive C) x) ;
-    }.
+Context `{Serializable Msg1} `{Serializable Setup1} `{Serializable State1} `{Serializable Error1}
+        `{Serializable Msg2} `{Serializable Setup2} `{Serializable State2} `{Serializable Error2}.
 
 (** The definition *)
 Record ContractMorphism 
-    (C  : Contract Setup  Msg  State  Error) 
-    (C' : Contract Setup' Msg' State' Error') := 
-    build_cm {
-        cm_init : InitCM C C' ;
-        cm_recv : RecvCM C C' ;
-    }.
+    (C1 : Contract Setup1 Msg1 State1 Error1) 
+    (C2 : Contract Setup2 Msg2 State2 Error2) := {
+    (* the components of a morphism f *)
+    msg_morph : Msg1 -> Msg2 ;
+    setup_morph : Setup1 -> Setup2 ;
+    state_morph : State1 -> State2 ;
+    error_morph : Error1 -> Error2 ;
+    (* coherence conditions *)
+    init_coherence : forall c ctx s, 
+        result_functor state_morph error_morph 
+            (init C1 c ctx s) = 
+        init C2 c ctx (setup_morph s) ;
+    recv_coherence : forall c ctx st op_msg, 
+        result_functor (fun '(st, l) => (state_morph st, l)) error_morph 
+            (receive C1 c ctx st op_msg) = 
+        receive C2 c ctx (state_morph st) (option_map msg_morph op_msg) ; }.
 
 End MorphismDefinition.
 
 
-Section MorphismUtilities.
-Context `{Serializable Msg}  `{Serializable Setup}  `{Serializable State}  `{Serializable Error}
-    `{Serializable Msg'} `{Serializable Setup'} `{Serializable State'} `{Serializable Error'}
-    {C : Contract Setup Msg State Error} {C' : Contract Setup' Msg' State' Error'}.
-
-Definition init_cm (f : ContractMorphism C C') : InitCM C C' := 
-    cm_init C C' f.
-Definition recv_cm (f : ContractMorphism C C') : RecvCM C C' := 
-    cm_recv C C' f.
-Definition id_fun (A : Type) : A -> A := @id A.
-
-(* the coherence conditions for constructing non-opaque morphisms *)
-Definition init_morphs_commute  
-    (init  : Chain -> ContractCallContext -> Setup  -> result State  Error)
-    (init' : Chain -> ContractCallContext -> Setup' -> result State' Error')
-    (init_inputs : Chain * ContractCallContext * Setup -> 
-        Chain * ContractCallContext * Setup') 
-    (init_outputs : result State Error -> result State' Error') :=
-    forall x : Chain * ContractCallContext * Setup,
-        uncurry_3 init' (init_inputs x) = 
-        init_outputs (uncurry_3 init x).
-
-Definition recv_morphs_commute 
-    (recv  : Chain -> ContractCallContext -> State  -> option Msg  -> 
-        result (State  * list ActionBody) Error)
-    (recv' : Chain -> ContractCallContext -> State' -> option Msg' -> 
-        result (State' * list ActionBody) Error')
-    (recv_inputs : Chain * ContractCallContext * State * option Msg -> 
-        Chain * ContractCallContext * State' * option Msg')
-    (recv_outputs : result (State * list ActionBody) Error -> 
-        result (State' * list ActionBody) Error') : Prop :=
-        forall (x : Chain * ContractCallContext * State * option Msg), 
-            uncurry_4 recv' (recv_inputs x) = 
-            recv_outputs (uncurry_4 recv x).
-
-End MorphismUtilities.
-
-
 (** The Identity Contract Morphism *)
 Section IdentityMorphism.
-Context { Setup Msg State Error : Type }
-  `{Serializable Msg}  `{Serializable Setup}  `{Serializable State} `{Serializable Error}.
+Context `{Serializable Msg} `{Serializable Setup} `{Serializable State} `{Serializable Error}.
 
-(* an opaque construction *)
-Definition id_cm_opaque (C : Contract Setup Msg State Error) : ContractMorphism C C.
-Proof.
-    constructor.
-    -   set (init_inputs  := id_fun (Chain * ContractCallContext * Setup)).
-        set (init_outputs := id_fun (result State Error)).
-        apply (build_init_cm C C init_inputs init_outputs).
-        intro. destruct x. destruct p.
-        unfold uncurry_3. 
-        unfold init_inputs. unfold init_outputs. 
-        unfold id_fun. simpl.
-        reflexivity.
-    -   set (recv_inputs  := id_fun (Chain * ContractCallContext * State * option Msg)).
-        set (recv_outputs := id_fun (result (State * list ActionBody) Error)).
-        apply (build_recv_cm C C recv_inputs recv_outputs).
-        intro. destruct x. repeat destruct p.
-        unfold uncurry_4. 
-        unfold recv_inputs. unfold recv_outputs. 
-        unfold id_fun. simpl.
-        reflexivity.
+Lemma init_coherence_id (C : Contract Setup Msg State Error) : 
+    forall c ctx s,
+    result_functor (@id State) (@id Error) (init C c ctx s) = 
+    init C c ctx s.
+Proof. 
+    intros.
+    unfold result_functor.
+    now destruct (init C c ctx s).
 Qed.
 
-(* an explicit construction *)
-Lemma init_commutes_id (C : Contract Setup Msg State Error) :
-    init_morphs_commute 
-        (init C) (init C) 
-        (id_fun (Chain * ContractCallContext * Setup)) 
-        (id_fun (result State Error)).
-Proof. now intro. Qed.
-
-Definition id_cm_init (C : Contract Setup Msg State Error) :
-    InitCM C C := {|
-        init_inputs  := id_fun (Chain * ContractCallContext * Setup) ;
-        init_outputs := id_fun (result State Error) ;
-        (* proof of commutativity *)
-        init_commutes := init_commutes_id C ;
-    |}.
-
-Lemma recv_commutes_id (C : Contract Setup Msg State Error) :
-    recv_morphs_commute 
-        (receive C) (receive C) 
-        (id_fun (Chain * ContractCallContext * State * option Msg)) 
-        (id_fun (result (State * list ActionBody) Error)).
-Proof. now intro. Qed.
-
-Definition id_cm_recv (C : Contract Setup Msg State Error) : RecvCM C C := {|
-        recv_inputs := id_fun (Chain * ContractCallContext * State * option Msg) ;
-        recv_outputs := id_fun (result (State * list ActionBody) Error) ;
-        (* proof of commutativity *)
-        recv_commutes := recv_commutes_id C ;
-    |}.
+Lemma recv_coherence_id (C : Contract Setup Msg State Error) : 
+    forall c ctx st op_msg, 
+    result_functor 
+        (fun '(st, l) => (@id State st, l)) (@id Error) 
+        (receive C c ctx st op_msg) = 
+    receive C c ctx (@id State st) (option_map (@id Msg) op_msg).
+Proof.
+    intros.
+    unfold result_functor, option_map. cbn.
+    destruct op_msg.
+    -   now destruct (receive C c ctx st (Some m)); try destruct t.
+    -   now destruct (receive C c ctx st None); try destruct t.
+Qed.
 
 (* * the identity morphism *)
 Definition id_cm (C : Contract Setup Msg State Error) : ContractMorphism C C := {|
-        cm_init := id_cm_init C ;
-        cm_recv := id_cm_recv C ;
+        (* components *)
+        msg_morph := @id Msg ; 
+        setup_morph := @id Setup ;
+        state_morph := @id State ; 
+        error_morph := @id Error ; 
+        (* coherence conditions *)
+        init_coherence := init_coherence_id C ; 
+        recv_coherence := recv_coherence_id C ;
     |}.
 
 End IdentityMorphism.
 
 (** Deriving equality of Contract Morphisms *)
 Section EqualityOfMorphisms.
-Context { Setup Setup' Msg Msg' State State' Error Error' : Type }
-    `{Serializable Msg}  `{Serializable Setup}  `{Serializable State}  `{Serializable Error}
-    `{Serializable Msg'} `{Serializable Setup'} `{Serializable State'} `{Serializable Error'}
-    {C : Contract Setup Msg State Error} {C' : Contract Setup' Msg' State' Error'}.
+Context `{Serializable Msg1} `{Serializable Setup1} `{Serializable State1} `{Serializable Error1}
+        `{Serializable Msg2} `{Serializable Setup2} `{Serializable State2} `{Serializable Error2}
+        {C1 : Contract Setup1 Msg1 State1 Error1} 
+        {C2 : Contract Setup2 Msg2 State2 Error2}.
 
-Lemma is_eq_cm :
-    forall (f g : ContractMorphism C C'), 
-    init_cm f = init_cm g -> 
-    recv_cm f = recv_cm g -> 
+Proposition eq_cm : 
+    forall (f g : ContractMorphism C1 C2),
+    (* if the components are equal ... *)
+    (msg_morph C1 C2 f) = (msg_morph C1 C2 g) -> 
+    (setup_morph C1 C2 f) = (setup_morph C1 C2 g) -> 
+    (state_morph C1 C2 f) = (state_morph C1 C2 g) -> 
+    (error_morph C1 C2 f) = (error_morph C1 C2 g) -> 
+    (* ... then the morphisms are equal *)
     f = g.
 Proof.
-    intros f g init_eq recv_eq.
-    destruct f. destruct g. f_equal.
-    - unfold init_cm in init_eq. 
-      now unfold cm_init in init_eq.
-    - unfold recv_cm in recv_eq. 
-      now unfold cm_recv in recv_eq.
-Qed.
-
-Lemma is_eq_cm_init :
-    forall (f g : ContractMorphism C C'),
-    (init_inputs C C' (init_cm f)) = (init_inputs C C' (init_cm g)) -> 
-    (init_outputs C C' (init_cm f)) = (init_outputs C C' (init_cm g)) -> 
-    init_cm f = init_cm g.
-Proof.
-    intros f g. 
-    destruct f, g. 
-    simpl.
-    destruct cm_init0, cm_init1. 
-    simpl. 
-    intros inputs_eq outputs_eq. 
-    subst. 
-    f_equal.
-    apply proof_irrelevance.
-Qed.
-
-Lemma is_eq_cm_recv :
-    forall (f g : ContractMorphism C C'),
-    (recv_inputs C C' (recv_cm f)) = (recv_inputs C C' (recv_cm g)) -> 
-    (recv_outputs C C' (recv_cm f)) = (recv_outputs C C' (recv_cm g)) -> 
-    recv_cm f = recv_cm g.
-Proof.
-    intros f g. 
-    destruct f, g. 
-    simpl.
-    destruct cm_recv0, cm_recv1. 
-    simpl.
-    intros inputs_eq outputs_eq. 
-    subst. 
-    f_equal.
+    intros f g.
+    destruct f, g.
+    cbn.
+    intros msg_eq set_eq st_eq err_eq.
+    subst.
+    f_equal;
     apply proof_irrelevance.
 Qed.
 
@@ -242,120 +125,102 @@ End EqualityOfMorphisms.
 
 (** An explicit construction of the composition of two morphisms *)
 Section MorphismComposition.
-Context { Setup Setup' Setup'' Msg Msg' Msg'' State State' State'' Error Error' Error'' : Type }
-  `{Serializable Msg} `{Serializable Setup} `{Serializable State} `{Serializable Error}
-  `{Serializable Msg'} `{Serializable Setup'} `{Serializable State'} `{Serializable Error'}
-  `{Serializable Msg''} `{Serializable Setup''} `{Serializable State''} `{Serializable Error''}
-  { C : Contract Setup Msg State Error } 
-  { C' : Contract Setup' Msg' State' Error' }
-  { C'' : Contract Setup'' Msg'' State'' Error'' }.
+Context `{Serializable Msg1} `{Serializable Setup1} `{Serializable State1} `{Serializable Error1}
+        `{Serializable Msg2} `{Serializable Setup2} `{Serializable State2} `{Serializable Error2}
+        `{Serializable Msg3} `{Serializable Setup3} `{Serializable State3} `{Serializable Error3}
+        { C1 : Contract Setup1 Msg1 State1 Error1 } 
+        { C2 : Contract Setup2 Msg2 State2 Error2 }
+        { C3 : Contract Setup3 Msg3 State3 Error3 }.
 
-(** The Init component *)
-Lemma compose_commutes_init (g : ContractMorphism C' C'') (f : ContractMorphism C  C') :
-    init_morphs_commute 
-        (init C) 
-        (init C'')
-        (compose (init_inputs  C' C'' (init_cm g)) (init_inputs  C C' (init_cm f)))
-        (compose (init_outputs C' C'' (init_cm g)) (init_outputs C C' (init_cm f))).
+Lemma compose_init_coh (g : ContractMorphism C2 C3) (f : ContractMorphism C1 C2) : 
+    let state_morph' := (compose (state_morph C2 C3 g) (state_morph C1 C2 f)) in 
+    let error_morph' := (compose (error_morph C2 C3 g) (error_morph C1 C2 f)) in 
+    let setup_morph' := (compose (setup_morph C2 C3 g) (setup_morph C1 C2 f)) in 
+    forall c ctx s, 
+        result_functor state_morph' error_morph'
+            (init C1 c ctx s) = 
+        init C3 c ctx (setup_morph' s).
 Proof.
-    unfold init_morphs_commute. intro. simpl.
-    rewrite (init_commutes C' C'' (init_cm g)).
-    rewrite (init_commutes C C' (init_cm f)). 
-    reflexivity.
+    intros.
+    unfold setup_morph'.
+    cbn.
+    rewrite <- (init_coherence C2 C3 g).
+    rewrite <- (init_coherence C1 C2 f).
+    unfold result_functor.
+    now destruct (init C1 c ctx s).
 Qed.
 
-(** The Recv component *)
-Lemma compose_commutes_recv (g : ContractMorphism C' C'') (f : ContractMorphism C  C') :
-    recv_morphs_commute 
-        (receive C)
-        (receive C'')
-        (compose (recv_inputs  C' C'' (recv_cm g)) (recv_inputs  C C' (recv_cm f)))
-        (compose (recv_outputs C' C'' (recv_cm g)) (recv_outputs C C' (recv_cm f))).
+Lemma compose_recv_coh (g : ContractMorphism C2 C3) (f : ContractMorphism C1 C2) : 
+    let state_morph' := (compose (state_morph C2 C3 g) (state_morph C1 C2 f)) in 
+    let error_morph' := (compose (error_morph C2 C3 g) (error_morph C1 C2 f)) in 
+    let msg_morph'   := (compose (msg_morph   C2 C3 g) (msg_morph   C1 C2 f)) in 
+    forall c ctx st op_msg, 
+        result_functor 
+            (fun '(st, l) => (state_morph' st, l)) error_morph' 
+            (receive C1 c ctx st op_msg) = 
+        receive C3 c ctx (state_morph' st) (option_map msg_morph' op_msg).
 Proof.
-    unfold recv_morphs_commute. intro. simpl.
-    rewrite (recv_commutes C' C'' (recv_cm g)). 
-    rewrite (recv_commutes C C' (recv_cm f)).
-    reflexivity.
+    intros.
+    pose proof (recv_coherence C2 C3 g).
+    pose proof (recv_coherence C1 C2 f).
+    unfold state_morph', msg_morph'.
+    cbn.
+    replace (option_map (compose (msg_morph C2 C3 g) (msg_morph C1 C2 f)) op_msg) 
+    with (option_map (msg_morph C2 C3 g) (option_map (msg_morph C1 C2 f) op_msg)).
+    2:{ now destruct op_msg. }
+    rewrite <- H11.
+    rewrite <- H12.
+    unfold result_functor.
+    now destruct (receive C1 c ctx st op_msg).
 Qed.
 
 (** Composition *)
-Definition composition_cm (g : ContractMorphism C' C'') (f : ContractMorphism C  C') 
-    : ContractMorphism C C'' := 
-    let compose_init := {|
-        init_inputs  := compose (init_inputs  C' C'' (init_cm g)) (init_inputs  C C' (init_cm f)) ;
-        init_outputs := compose (init_outputs C' C'' (init_cm g)) (init_outputs C C' (init_cm f)) ;
-        (* proof of commutativity *)
-        init_commutes := compose_commutes_init g f ;
-    |} in 
-    let compose_recv := {|
-        recv_inputs  := compose (recv_inputs  C' C'' (recv_cm g)) (recv_inputs  C C' (recv_cm f)) ;
-        recv_outputs := compose (recv_outputs C' C'' (recv_cm g)) (recv_outputs C C' (recv_cm f)) ;
-        (* proof of commutativity *)
-        recv_commutes := compose_commutes_recv g f ;
-    |} in 
-    {|
-        cm_init := compose_init ;
-        cm_recv := compose_recv ;
+Definition composition_cm (g : ContractMorphism C2 C3) (f : ContractMorphism C1 C2) : 
+    ContractMorphism C1 C3 := {| 
+    (* the components *)
+    msg_morph   := compose (msg_morph   C2 C3 g) (msg_morph   C1 C2 f) ; 
+    setup_morph := compose (setup_morph C2 C3 g) (setup_morph C1 C2 f) ; 
+    state_morph := compose (state_morph C2 C3 g) (state_morph C1 C2 f) ; 
+    error_morph := compose (error_morph C2 C3 g) (error_morph C1 C2 f) ; 
+    (* the coherence results *)
+    init_coherence := compose_init_coh g f ; 
+    recv_coherence := compose_recv_coh g f ; 
     |}.
 
 End MorphismComposition.
 
 Section MorphismCompositionResults.
-Context { Setup Setup' Setup'' Setup''' Msg Msg' Msg'' Msg''' 
-          State State' State'' State''' Error Error' Error'' Error''' : Type }
-    `{Serializable Msg} `{Serializable Setup} `{Serializable State} `{Serializable Error}
-    `{Serializable Msg'} `{Serializable Setup'} `{Serializable State'} `{Serializable Error'}
-    `{Serializable Msg''} `{Serializable Setup''} `{Serializable State''} `{Serializable Error''}
-    `{Serializable Msg'''} `{Serializable Setup'''} `{Serializable State'''} `{Serializable Error'''}
-    { C : Contract Setup Msg State Error } 
-    { C' : Contract Setup' Msg' State' Error' }
-    { C'' : Contract Setup'' Msg'' State'' Error'' }
-    { C''' : Contract Setup''' Msg''' State''' Error''' }.
+Context `{Serializable Msg1} `{Serializable Setup1} `{Serializable State1} `{Serializable Error1}
+        `{Serializable Msg2} `{Serializable Setup2} `{Serializable State2} `{Serializable Error2}
+        `{Serializable Msg3} `{Serializable Setup3} `{Serializable State3} `{Serializable Error3}
+        `{Serializable Msg4} `{Serializable Setup4} `{Serializable State4} `{Serializable Error4}
+        { C1 : Contract Setup1 Msg1 State1 Error1 } 
+        { C2 : Contract Setup2 Msg2 State2 Error2 }
+        { C3 : Contract Setup3 Msg3 State3 Error3 }
+        { C4 : Contract Setup4 Msg4 State4 Error4 }.
 
 (** Composition with the Identity morphism is trivial *)
-Proposition composition_id_cm_left :
-    forall (f : ContractMorphism C C'), 
-    (composition_cm (id_cm C') f) = f.
+Proposition composition_id_cm_left (f : ContractMorphism C1 C2) :
+    composition_cm (id_cm C2) f = f.
 Proof.
-    intros. 
-    unfold composition_cm, id_cm. 
-    simpl.
-    apply is_eq_cm; simpl.
-    -   apply (is_eq_cm_init (composition_cm (id_cm C') f) f); auto.
-    -   apply (is_eq_cm_recv (composition_cm (id_cm C') f) f); auto.
+    now apply eq_cm.
 Qed.
 
-Proposition composition_id_cm_right :
-    forall (f : ContractMorphism C C'), 
-    (composition_cm f (id_cm C)) = f.
+Proposition composition_id_cm_right (f : ContractMorphism C1 C2) :
+    composition_cm f (id_cm C1) = f.
 Proof.
-    intros. 
-    unfold composition_cm, id_cm. 
-    simpl.
-    apply is_eq_cm; simpl. 
-    + apply (is_eq_cm_init (composition_cm f (id_cm C)) f); auto.
-    + apply (is_eq_cm_recv (composition_cm f (id_cm C)) f); auto.
+    now apply eq_cm.
 Qed.
 
 (** Composition is associative *)
-Proposition composition_assoc_cm :
-    forall 
-    (f : ContractMorphism C C') 
-    (g : ContractMorphism C' C'') 
-    (h : ContractMorphism C'' C'''), 
+Proposition composition_assoc_cm
+    (f : ContractMorphism C1 C2) 
+    (g : ContractMorphism C2 C3) 
+    (h : ContractMorphism C3 C4) :
     composition_cm h (composition_cm g f) =
     composition_cm (composition_cm h g) f.
 Proof.
-    intros.
-    unfold composition_cm. simpl. apply is_eq_cm.
-    -   now apply 
-        (is_eq_cm_init 
-            (composition_cm h (composition_cm g f))
-            (composition_cm (composition_cm h g) f)).
-    -   now apply 
-        (is_eq_cm_recv 
-            (composition_cm h (composition_cm g f))
-            (composition_cm (composition_cm h g) f)).
+    now apply eq_cm.
 Qed.
 
 End MorphismCompositionResults.
@@ -363,88 +228,70 @@ End MorphismCompositionResults.
 
 (** We will treat various type of contract morphisms, starting with isomorphisms. *)
 Section IsomorphismDefinition.
-Context { Setup Setup' Msg Msg' State State' Error Error' : Type }
-`{Serializable Msg}  `{Serializable Setup}  `{Serializable State}  `{Serializable Error}
-`{Serializable Msg'} `{Serializable Setup'} `{Serializable State'} `{Serializable Error'}
-{C : Contract Setup Msg State Error} {C' : Contract Setup' Msg' State' Error'}.
+Context `{Serializable Msg1} `{Serializable Setup1} `{Serializable State1} `{Serializable Error1}
+        `{Serializable Msg2} `{Serializable Setup2} `{Serializable State2} `{Serializable Error2}
+        {C1 : Contract Setup1 Msg1 State1 Error1} 
+        {C2 : Contract Setup2 Msg2 State2 Error2}.
 
 Definition is_iso {A B : Type} (f : A -> B) (g : B -> A) : Prop := 
     compose g f = @id A /\ compose f g = @id B.
 
 Lemma is_iso_reflexive {A B : Type} (f : A -> B) (g : B -> A) : 
     is_iso f g -> is_iso g f.
-Proof. unfold is_iso. intro H_is_iso. now destruct H_is_iso. Qed.
+Proof. 
+    unfold is_iso. 
+    intro H_is_iso. 
+    now destruct H_is_iso. 
+Qed.
 
-Definition is_iso_cm 
-    (f : ContractMorphism C C')
-    (g : ContractMorphism C' C) : Prop := 
-    composition_cm g f = id_cm C /\ 
-    composition_cm f g = id_cm C'.
+Definition is_iso_cm (f : ContractMorphism C1 C2) (g : ContractMorphism C2 C1) : Prop :=
+    composition_cm g f = id_cm C1 /\
+    composition_cm f g = id_cm C2.
 
 Lemma iso_cm_components :
-    forall (f : ContractMorphism C C') (g : ContractMorphism C' C),
-    is_iso (init_inputs  C C' (init_cm f)) (init_inputs  C' C (init_cm g)) /\
-    is_iso (init_outputs C C' (init_cm f)) (init_outputs C' C (init_cm g)) /\
-    is_iso (recv_inputs  C C' (recv_cm f)) (recv_inputs  C' C (recv_cm g)) /\
-    is_iso (recv_outputs C C' (recv_cm f)) (recv_outputs C' C (recv_cm g)) 
+    forall (f : ContractMorphism C1 C2) (g : ContractMorphism C2 C1),
+    is_iso (msg_morph   C1 C2 f) (msg_morph   C2 C1 g) /\
+    is_iso (setup_morph C1 C2 f) (setup_morph C2 C1 g) /\
+    is_iso (state_morph C1 C2 f) (state_morph C2 C1 g) /\
+    is_iso (error_morph C1 C2 f) (error_morph C2 C1 g)
     <->
     is_iso_cm f g.
 Proof.
-    intros f g. unfold is_iso. unfold iff. split.
-    -   intro E. 
-        destruct E as [iso_i_inputs E'].
-        destruct iso_i_inputs as [iso_i_inputs1 iso_i_inputs2].
-        destruct E' as [iso_i_outputs E''].
-        destruct iso_i_outputs as [iso_i_outputs1 iso_i_outputs2].
-        destruct E'' as [iso_r_inputs iso_r_outputs].
-        destruct iso_r_inputs as [iso_r_inputs1 iso_r_inputs2].
-        destruct iso_r_outputs as [iso_r_outputs1 iso_r_outputs2].
-        unfold is_iso_cm. unfold composition_cm. unfold id_cm. 
-        unfold id_cm_init. unfold id_cm_recv. unfold id_fun. 
-        split.
-        +   apply is_eq_cm.
-            * apply is_eq_cm_init; simpl.
-                ** exact iso_i_inputs1. 
-                ** exact iso_i_outputs1.
-            * apply is_eq_cm_recv; simpl.
-                ** exact iso_r_inputs1.
-                ** exact iso_r_outputs1.
-        +   apply is_eq_cm.
-            *  apply is_eq_cm_init; simpl. 
-                ** exact iso_i_inputs2. 
-                ** exact iso_i_outputs2.
-            *  apply is_eq_cm_recv; simpl.
-                ** exact iso_r_inputs2.
-                ** exact iso_r_outputs2. 
-    -   unfold is_iso_cm. unfold composition_cm.  unfold id_cm. 
-        unfold id_cm_init. unfold id_cm_recv. unfold id_fun.
-        intro is_iso_H. destruct is_iso_H as [is_iso_H1 is_iso_H2].
-        inversion is_iso_H1. inversion is_iso_H2.
-        auto.
+    intros f g. 
+    unfold is_iso. 
+    unfold iff. 
+    split.
+    (* -> *)
+    -   intro H_iso.
+        unfold is_iso_cm.
+        split; now apply eq_cm.
+    (* <- *)
+    -   unfold is_iso_cm, composition_cm, id_cm.
+        now intro H_iso.
 Qed.
 
 End IsomorphismDefinition.
 
 
 Section Isomorphisms.
-Context { Setup Setup' Setup'' Setup''' Msg Msg' Msg'' Msg''' State State' State'' State''' 
-            Error Error' Error'' Error''' : Type }
-    `{Serializable Msg} `{Serializable Setup} `{Serializable State} `{Serializable Error}
-    `{Serializable Msg'} `{Serializable Setup'} `{Serializable State'} `{Serializable Error'}
-    `{Serializable Msg''} `{Serializable Setup''} `{Serializable State''} `{Serializable Error''}
-    `{Serializable Msg'''} `{Serializable Setup'''} `{Serializable State'''} `{Serializable Error'''}
-    { C : Contract Setup Msg State Error } 
-    { C' : Contract Setup' Msg' State' Error' }
-    { C'' : Contract Setup'' Msg'' State'' Error'' }
-    { C''' : Contract Setup''' Msg''' State''' Error''' }.
+Context `{Serializable Msg1} `{Serializable Setup1} `{Serializable State1} `{Serializable Error1}
+        `{Serializable Msg2} `{Serializable Setup2} `{Serializable State2} `{Serializable Error2}.
 
+(** An equality predicate on contracts *)
 Definition contracts_isomorphic 
-    (C : Contract Setup Msg State Error)
-    (C' : Contract Setup' Msg' State' Error') : Prop := 
-    exists (f : ContractMorphism C C') (g : ContractMorphism C' C),
+    (C1 : Contract Setup1 Msg1 State1 Error1)
+    (C2 : Contract Setup2 Msg2 State2 Error2) : Prop := 
+    exists (f : ContractMorphism C1 C2) (g : ContractMorphism C2 C1),
     is_iso_cm f g.
 
-Lemma iso_cm_reflexive (f : ContractMorphism C C') (g : ContractMorphism C' C) : 
+Context `{Serializable Msg3} `{Serializable Setup3} `{Serializable State3} `{Serializable Error3}
+        `{Serializable Msg4} `{Serializable Setup4} `{Serializable State4} `{Serializable Error4}
+        { C1 : Contract Setup1 Msg1 State1 Error1 } 
+        { C2 : Contract Setup2 Msg2 State2 Error2 }
+        { C3 : Contract Setup3 Msg3 State3 Error3 }
+        { C4 : Contract Setup4 Msg4 State4 Error4 }.
+
+Lemma iso_cm_reflexive (f : ContractMorphism C1 C2) (g : ContractMorphism C2 C1) : 
     is_iso_cm f g -> 
     is_iso_cm g f.
 Proof.
@@ -461,423 +308,80 @@ Proof.
 Qed.
 
 Lemma composition_iso_cm 
-    (f : ContractMorphism C C')
-    (g : ContractMorphism C' C'')
-    (f' : ContractMorphism C' C)
-    (g' : ContractMorphism C'' C') :
-    is_iso_cm f f' -> 
-    is_iso_cm g g' -> 
-    is_iso_cm (composition_cm g f) (composition_cm f' g').
+    (f1 : ContractMorphism C1 C2)
+    (g1 : ContractMorphism C2 C3)
+    (f2 : ContractMorphism C2 C1)
+    (g2 : ContractMorphism C3 C2) :
+    is_iso_cm f1 f2 -> 
+    is_iso_cm g1 g2 -> 
+    is_iso_cm (composition_cm g1 f1) (composition_cm f2 g2).
 Proof.
     unfold is_iso_cm.
     intros iso_f iso_g. 
     destruct iso_f as [iso_f1 iso_f2].
     destruct iso_g as [iso_g1 iso_g2].
-    split.
-    -   rewrite composition_assoc_cm. 
-        rewrite <- (composition_assoc_cm g g' f').
-        rewrite iso_g1. rewrite (composition_id_cm_right f'). exact iso_f1.
-    -   rewrite composition_assoc_cm.
-        rewrite <- (composition_assoc_cm f' f g).
-        rewrite iso_f2. rewrite (composition_id_cm_right g). exact iso_g2.
+    split; rewrite composition_assoc_cm.
+    -   rewrite <- (composition_assoc_cm g1 g2 f2).
+        rewrite iso_g1. 
+        now rewrite (composition_id_cm_right f2).
+    -   rewrite <- (composition_assoc_cm f2 f1 g1).
+        rewrite iso_f2. 
+        now rewrite (composition_id_cm_right g1).
 Qed.
 
 End Isomorphisms.
 
-
+Axiom todo : string -> forall {A}, A.
 (** Now, onto injections *)
 Section Injections.
-Context { Setup Setup' Msg Msg' State State' Error Error' : Type }
-    `{Serializable Msg}  `{Serializable Setup}  `{Serializable State}  `{Serializable Error}
-    `{Serializable Msg'} `{Serializable Setup'} `{Serializable State'} `{Serializable Error'}
-    {C : Contract Setup Msg State Error} {C' : Contract Setup' Msg' State' Error'}.
+Context `{Serializable Msg1} `{Serializable Setup1} `{Serializable State1} `{Serializable Error1}
+        `{Serializable Msg2} `{Serializable Setup2} `{Serializable State2} `{Serializable Error2}
+        {C1 : Contract Setup1 Msg1 State1 Error1} 
+        {C2 : Contract Setup2 Msg2 State2 Error2}.
 
 Definition is_inj {A B : Type} (f : A -> B) : Prop := 
     forall (a a' : A), f a = f a' -> a = a'.
 
-Definition is_inj_cm 
-    (f : ContractMorphism C C') : Prop := 
-    (* init morphisms inject *)
-    is_inj (init_inputs  C C' (init_cm f)) /\
-    (* recv morphisms inject *)
-    is_inj (recv_inputs  C C' (recv_cm f)).
+Definition is_inj_cm (f : ContractMorphism C1 C2) : Prop := 
+    todo "".
 
 Definition contract_embeds : Prop := 
-    exists (f : ContractMorphism C C'), is_inj_cm f.
+    exists (f : ContractMorphism C1 C2), is_inj_cm f.
 
 End Injections.
 
 
 (** Finally, we treat surjections, or quotients *)
 Section Surjections.
-Context { Setup Setup' Msg Msg' State State' Error Error' : Type }
-    `{Serializable Msg}  `{Serializable Setup}  `{Serializable State}  `{Serializable Error}
-    `{Serializable Msg'} `{Serializable Setup'} `{Serializable State'} `{Serializable Error'}
-    {C : Contract Setup Msg State Error} {C' : Contract Setup' Msg' State' Error'}.
+Context `{Serializable Msg1} `{Serializable Setup1} `{Serializable State1} `{Serializable Error1}
+        `{Serializable Msg2} `{Serializable Setup2} `{Serializable State2} `{Serializable Error2}
+        {C1 : Contract Setup1 Msg1 State1 Error1} 
+        {C2 : Contract Setup2 Msg2 State2 Error2}.
 
 Definition is_surj {A B : Type} (f : A -> B) : Prop := 
     forall (b : B), exists (a : A), f a = b.
 
-Definition is_surj_cm (f : ContractMorphism C C') : Prop := 
-    (* init morphisms surject *)
-    is_surj (init_inputs C C' (init_cm f)) /\
-    (* recv morphisms surject *)
-    is_surj (recv_inputs C C' (recv_cm f)).
+Definition is_surj_cm (f : ContractMorphism C1 C2) : Prop := todo "".
 
 Definition contract_surjects : Prop := 
-    exists (f : ContractMorphism C C'), is_surj_cm f.
+    exists (f : ContractMorphism C1 C2), is_surj_cm f.
 
 End Surjections.
 
 (** TODO EXACTNESS *)
+Section Exactness.
+Context `{Serializable Msg1} `{Serializable Setup1} `{Serializable State1} `{Serializable Error1}
+        `{Serializable Msg2} `{Serializable Setup2} `{Serializable State2} `{Serializable Error2}
+        `{Serializable Msg3} `{Serializable Setup3} `{Serializable State3} `{Serializable Error3}
+        { C1 : Contract Setup1 Msg1 State1 Error1 } 
+        { C2 : Contract Setup2 Msg2 State2 Error2 }
+        { C3 : Contract Setup3 Msg3 State3 Error3 }.
 
 
-(** The definition of contract morphisms is fairly general, and 
-    somewhat difficult to work with. As we proceed, we will use 
-    simple contract morphisms, which can be decomposed as functions 
-    between state, msg, setup, and error types along with the corresponding
-    coherence result.
-    
-    This simpler structure will allow us to lift contract morphisms into
-    a transformation of chainstate and trace.
-    
-    Note that these simpler morphisms do not modify balances or emitted 
-    actions. Future work could include generalizing the lifting result
-    to allow for more contract morphisms.
-*)
-Section SimpleContractMorphism.
-Context { Setup Setup' Msg Msg' State State' Error Error' : Type }
-    `{Serializable Msg}  `{Serializable Setup}  `{Serializable State}  `{Serializable Error}
-    `{Serializable Msg'} `{Serializable Setup'} `{Serializable State'} `{Serializable Error'}.
-
-Definition result_functor {T T' E E' : Type} : (T -> T') -> (E -> E') -> result T E -> result T' E' :=
-    fun (f_t : T -> T') (f_e : E -> E') (res : result T E) => 
-    match res with | Ok t => Ok (f_t t) | Err e => Err (f_e e) end.
-
-(** The definition of a simple contract morphism *)
-Record simple_cm 
-    (C : Contract Setup Msg State Error) (C' : Contract Setup' Msg' State' Error') := {
-    (* the components of a simple morphism f *)
-    msg_morph : Msg -> Msg' ;
-    setup_morph : Setup -> Setup' ;
-    state_morph : State -> State' ;
-    error_morph : Error -> Error' ;
-    (* coherence conditions *)
-    init_coherence : forall c ctx s, 
-        result_functor state_morph error_morph (init C c ctx s) = 
-        init C' c ctx (setup_morph s) ;
-    recv_coherence : forall c ctx st op_msg, 
-        result_functor (fun '(st, l) => (state_morph st, l)) error_morph (receive C c ctx st op_msg) = 
-        receive C' c ctx (state_morph st) (option_map msg_morph op_msg) ; }.
-
-Context {C1 : Contract Setup Msg State Error} {C2 : Contract Setup' Msg' State' Error'}.
-
-(** We explicitly construct the components *)
-(* the init component *)
-Lemma init_commutes_simple 
-    (* the components of f *)
-    (setup_morph : Setup -> Setup')
-    (state_morph : State -> State')
-    (error_morph : Error -> Error')
-    (* coherence conditions *)
-    (init_coherence : forall c ctx s, 
-        result_functor state_morph error_morph (init C1 c ctx s) = init C2 c ctx (setup_morph s)) : 
-    init_morphs_commute 
-        (init C1) (init C2)
-        (fun (x : Chain * ContractCallContext * Setup) => 
-            let '(c, ctx, s) := x in (c, ctx, setup_morph s))
-        (result_functor state_morph error_morph).
-Proof.
-    unfold init_morphs_commute. 
-    intro. destruct x. destruct p.
-    unfold uncurry_3. simpl.
-    now rewrite <- (init_coherence c c0 s).
-Qed.
-
-Definition simple_cm_init 
-    (* the components of f *)
-    (setup_morph : Setup -> Setup')
-    (state_morph : State -> State')
-    (error_morph : Error -> Error')
-    (* coherence conditions *)
-    (init_coherence : forall c ctx s, 
-        result_functor state_morph error_morph (init C1 c ctx s) = init C2 c ctx (setup_morph s)) : 
-    InitCM C1 C2 := {| 
-        init_inputs := (fun (x : Chain * ContractCallContext * Setup) => 
-        let '(c, ctx, s) := x in (c, ctx, setup_morph s)) ; 
-        init_outputs := (result_functor state_morph error_morph) ; 
-        init_commutes := init_commutes_simple setup_morph state_morph error_morph init_coherence ;
-    |}.
-
-(* the recv component *)
-Lemma recv_commutes_simple 
-    (* the components of f *)
-    (msg_morph   : Msg   -> Msg')
-    (state_morph : State -> State')
-    (error_morph : Error -> Error')
-    (* coherence conditions *)
-    (recv_coherence : forall c ctx st op_msg, 
-        result_functor (fun '(st, l) => (state_morph st, l)) error_morph (receive C1 c ctx st op_msg) 
-        = (receive C2) c ctx (state_morph st) (option_map msg_morph op_msg)) : 
-    recv_morphs_commute
-        (receive C1) (receive C2)
-        (fun (x : Chain * ContractCallContext * State * option Msg) => 
-            let '(c, ctx, st, op_msg) := x in (c, ctx, state_morph st, option_map msg_morph op_msg))
-        (result_functor (fun '(st, l) => (state_morph st, l)) error_morph).
-Proof.
-    unfold recv_morphs_commute. 
-    intro. 
-    destruct x. 
-    repeat destruct p.
-    unfold uncurry_4. 
-    simpl.
-    now rewrite <- recv_coherence.
-Qed.
-
-Definition simple_cm_recv 
-    (* the components of f *)
-    (msg_morph   : Msg   -> Msg')
-    (state_morph : State -> State')
-    (error_morph : Error -> Error')
-    (* coherence conditions *)
-    (recv_coherence : forall c ctx st op_msg, 
-        result_functor (fun '(st, l) => (state_morph st, l)) error_morph (receive C1 c ctx st op_msg) 
-        = receive C2 c ctx (state_morph st) (option_map msg_morph op_msg)) : 
-    RecvCM C1 C2 := {| 
-        recv_inputs := 
-            (fun (x : Chain * ContractCallContext * State * option Msg) => 
-                let '(c, ctx, st, op_msg) := x in (c, ctx, state_morph st, option_map msg_morph op_msg)) ; 
-        recv_outputs := 
-            (result_functor (fun '(st, l) => (state_morph st, l)) error_morph) ; 
-        recv_commutes := recv_commutes_simple msg_morph state_morph error_morph recv_coherence ;
-    |}.
-
-(* the simple contract morphism *)
-Definition simple_cm_construct
-    (* the components of f *)
-    (msg_morph   : Msg   -> Msg')
-    (setup_morph : Setup -> Setup')
-    (state_morph : State -> State')
-    (error_morph : Error -> Error')
-    (* coherence conditions *)
-    (init_coherence : forall c ctx s, 
-        result_functor state_morph error_morph (init C1 c ctx s) = init C2 c ctx (setup_morph s))
-    (recv_coherence : forall c ctx st op_msg, 
-        (result_functor (fun '(st, l) => (state_morph st, l)) error_morph) 
-            (receive C1 c ctx st op_msg) = 
-        receive C2 c ctx (state_morph st) (option_map msg_morph op_msg)) : 
-    ContractMorphism C1 C2 := {| 
-        cm_init := simple_cm_init setup_morph state_morph error_morph init_coherence ;
-        cm_recv := simple_cm_recv msg_morph   state_morph error_morph recv_coherence ;
-    |}.
-
-Definition simple_cm_to_cm (f : simple_cm C1 C2) : ContractMorphism C1 C2 := 
-    simple_cm_construct (msg_morph C1 C2 f) (setup_morph C1 C2 f) (state_morph C1 C2 f) 
-        (error_morph C1 C2 f) (init_coherence C1 C2 f) (recv_coherence C1 C2 f).
-
-(* a predicate to indicate that a contract morphism is simple *)
-Definition is_simple_cm
-    (f : ContractMorphism C1 C2) : Prop := 
-    exists 
-    (* the components of f *)
-    (msg_morph   : Msg   -> Msg')
-    (setup_morph : Setup -> Setup')
-    (state_morph : State -> State')
-    (error_morph : Error -> Error')
-    (* coherence conditions *)
-    (init_coherence : forall c ctx s, 
-        result_functor state_morph error_morph (init C1 c ctx s) = init C2 c ctx (setup_morph s))
-    (recv_coherence : forall c ctx st op_msg, 
-        (result_functor (fun '(st, l) => (state_morph st, l)) error_morph) 
-            (receive C1 c ctx st op_msg) = 
-        receive C2 c ctx (state_morph st) (option_map msg_morph op_msg)),
-    f = simple_cm_construct msg_morph setup_morph state_morph error_morph init_coherence recv_coherence.
-
-(* a trivial lemma for convenience *)
-Lemma simple_cm_is_simple
-    (* the components of f *)
-    {msg_morph   : Msg   -> Msg'}
-    {setup_morph : Setup -> Setup'}
-    {state_morph : State -> State'}
-    {error_morph : Error -> Error'}
-    (* coherence conditions *)
-    {init_coherence : forall c ctx s, 
-        (result_functor state_morph error_morph) (init C1 c ctx s) = init C2 c ctx (setup_morph s)}
-    {recv_coherence : forall c ctx st op_msg, 
-        (result_functor (fun '(st, l) => (state_morph st, l)) error_morph) 
-            (receive C1 c ctx st op_msg) = 
-        receive C2 c ctx (state_morph st) (option_map msg_morph op_msg)} : 
-    is_simple_cm (simple_cm_construct msg_morph setup_morph state_morph error_morph init_coherence recv_coherence).
-Proof. 
-    unfold is_simple_cm.
-    exists msg_morph. exists setup_morph. exists state_morph. 
-    exists error_morph. exists init_coherence. exists recv_coherence.
-    auto.
-Qed.
-
-End SimpleContractMorphism.
+(** TODO in light of e.g.s *)
 
 
-Section SimpleContractMorphism_Composition.
-
-Context { Setup Setup' Setup'' Msg Msg' Msg'' State State' State'' Error Error' Error'' : Type }
-    `{Serializable Msg}    `{Serializable Setup}    `{Serializable State}    `{Serializable Error}
-    `{Serializable Msg'}   `{Serializable Setup'}   `{Serializable State'}   `{Serializable Error'}
-    `{Serializable Msg''}  `{Serializable Setup''}  `{Serializable State''}  `{Serializable Error''}
-    { C : Contract Setup Msg State Error } 
-    { C' : Contract Setup' Msg' State' Error' }
-    { C'' : Contract Setup'' Msg'' State'' Error'' }.
-
-(* simple morphisms compose to simple morphisms *)
-Lemma composition_simple_cm
-    (g : ContractMorphism C' C'')
-    (f : ContractMorphism C  C') :
-    is_simple_cm g -> 
-    is_simple_cm f -> 
-    is_simple_cm (composition_cm g f).
-Proof. 
-    unfold is_simple_cm.
-    intros g_simple f_simple.
-    (* extract functions from g *)
-    destruct g_simple as [g_msg [g_setup [g_state [g_error [g_init [g_recv g_simple]]]]]].
-    (* extract functions from f *)
-    destruct f_simple as [f_msg [f_setup [f_state [f_error [f_init [f_recv f_simple]]]]]].
-    (* construct g \circ f *)
-    exists (compose g_msg f_msg).
-    exists (compose g_setup f_setup).
-    exists (compose g_state f_state).
-    exists (compose g_error f_error).
-    (* proof of init coherence *)
-    assert (forall (c : Chain) (ctx : ContractCallContext) (s : Setup),
-        result_functor
-            (compose g_state f_state)
-            (compose g_error f_error) (init C c ctx s) =
-        init C'' c ctx (compose g_setup f_setup s))
-    as gf_init.
-    { intros. simpl.
-    rewrite <- g_init.
-    rewrite <- f_init.
-    destruct (init C c ctx s); auto. }
-    exists gf_init.
-    (* proof of recv coherence *)
-    assert (forall (c : Chain) (ctx : ContractCallContext) (st : State) (op_msg : option Msg),
-        result_functor 
-            (fun '(st, l) => (compose g_state f_state st, l))
-            (compose g_error f_error) (receive C c ctx st op_msg) =
-        receive C'' c ctx (compose g_state f_state st) (option_map (compose g_msg f_msg) op_msg))
-    as gf_recv.
-    {   intros. simpl.
-        replace (option_map (compose g_msg f_msg) op_msg) with (option_map g_msg (option_map f_msg op_msg)).
-        rewrite <- g_recv.
-        rewrite <- f_recv.
-        destruct (receive C c ctx st op_msg); simpl; auto. 
-        destruct t; auto.
-        destruct op_msg; auto. }
-    exists gf_recv.
-    (* rewrite the LHS *)
-    rewrite g_simple. 
-    rewrite f_simple.
-    unfold composition_cm. 
-    unfold simple_cm_construct.
-    apply is_eq_cm.
-    - apply is_eq_cm_init. 
-        +   simpl. 
-            apply functional_extensionality. 
-            intro. 
-            destruct x. 
-            destruct p. 
-            auto.
-        +   simpl. 
-            apply functional_extensionality.
-            intro. 
-            destruct x; auto.
-    - apply is_eq_cm_recv.
-        +   simpl. 
-            apply functional_extensionality.
-            intro. 
-            destruct x. 
-            repeat destruct p. 
-            simpl. 
-            destruct o; auto.
-        +   simpl. 
-            apply functional_extensionality.
-            intro. 
-            destruct x. 
-            destruct t. 
-            all: auto.
-Qed.
-
-End SimpleContractMorphism_Composition.
-
-
-Section IdSimple.
-Context { Setup Msg State Error : Type }
-    `{Serializable Msg}  `{Serializable Setup}  `{Serializable State} `{Serializable Error}.
-
-(* the identity is a simple morphism *)
-Lemma identity_simple 
-    (C : Contract Setup Msg State Error) : 
-    is_simple_cm (id_cm C).
-Proof. 
-    unfold is_simple_cm.
-    exists (id_fun Msg).
-    exists (id_fun Setup).
-    exists (id_fun State).
-    exists (id_fun Error).
-    assert (forall (c : Chain) (ctx : ContractCallContext) (s : Setup),
-            result_functor (id_fun State) (id_fun Error) (init C c ctx s) =
-            init C c ctx (id_fun Setup s))
-    as id_init.
-    {   intros. 
-        unfold id_fun; simpl. 
-        now destruct (init C c ctx s). }
-    exists id_init.
-    assert (forall (c : Chain) (ctx : ContractCallContext) (st : State) (op_msg : option Msg),
-            result_functor (fun '(st, l) => (id_fun State st, l)) (id_fun Error) (receive C c ctx st op_msg) =
-            receive C c ctx (id_fun State st) (option_map (id_fun Msg) op_msg))
-    as id_recv.
-    {   intros. 
-        unfold option_map, id_fun.
-        destruct op_msg.
-        -   simpl.
-            now destruct (receive C c ctx st (Some m)).
-        -   simpl.
-            now destruct (receive C c ctx st None). }
-    exists id_recv.
-    (* prove that id_cm C is simple wrt the above definitions *)
-    unfold id_cm. 
-    unfold simple_cm_construct.
-    apply is_eq_cm.
-    - apply is_eq_cm_init.
-        +   simpl. 
-            unfold id_fun. 
-            apply functional_extensionality. 
-            intro. 
-            destruct x. 
-            destruct p. 
-            auto.
-        +   simpl. 
-            unfold id_fun. 
-            apply functional_extensionality. 
-            intro. 
-            destruct x; auto.
-    - apply is_eq_cm_recv.
-        +   simpl. 
-            unfold id_fun. 
-            apply functional_extensionality. 
-            intro. 
-            destruct x. 
-            repeat destruct p. 
-            now destruct o.
-        +   simpl. 
-            unfold id_fun. 
-            apply functional_extensionality. 
-            intro. 
-            now destruct x; auto.
-Qed.
-
-End IdSimple.
-
+End Exactness.
 
 
 (** Morphism Induction: 
@@ -888,80 +392,80 @@ Section MorphismInduction.
 (** Define the notion of a contract's trace, which is a chained list of successful
     contract calls which mimics the blockchain. *)
 Section ContractTrace.
-    Context { Setup Msg State Error : Type }
-            `{Serializable Msg} `{Serializable Setup} `{Serializable State} `{Serializable Error}.
+Context { Setup Msg State Error : Type }
+        `{Serializable Msg} `{Serializable Setup} `{Serializable State} `{Serializable Error}.
 
-    (* Notions of contract state stepping forward *)
-    Record ContractStep (C : Contract Setup Msg State Error)
-        (prev_cstate : State) (next_cstate : State) := 
-        build_contract_step {
-        seq_chain : Chain ;
-        seq_ctx : ContractCallContext ;
-        seq_msg : option Msg ;
-        seq_new_acts : list ActionBody ;
-        (* we can call receive successfully *)
-        recv_some_step : 
-            receive C seq_chain seq_ctx prev_cstate seq_msg = Ok (next_cstate, seq_new_acts) ;
-    }.
+(* Notions of contract state stepping forward *)
+Record ContractStep (C : Contract Setup Msg State Error)
+    (prev_cstate : State) (next_cstate : State) := 
+    build_contract_step {
+    seq_chain : Chain ;
+    seq_ctx : ContractCallContext ;
+    seq_msg : option Msg ;
+    seq_new_acts : list ActionBody ;
+    (* we can call receive successfully *)
+    recv_some_step : 
+        receive C seq_chain seq_ctx prev_cstate seq_msg = Ok (next_cstate, seq_new_acts) ;
+}.
 
-    Definition ContractTrace (C : Contract Setup Msg State Error) := 
-        ChainedList State (ContractStep C).
+Definition ContractTrace (C : Contract Setup Msg State Error) := 
+    ChainedList State (ContractStep C).
 
-    (* TODO some notion of reachability which involves an `init_state` to replace 
-        into left_cm_induction *)
+(* TODO some notion of reachability which involves an `init_state` to replace 
+    into left_cm_induction *)
 
-    Definition cstate_reachable (C : Contract Setup Msg State Error) (cstate : State) : Prop := 
-        exists init_cstate,
-        (* init_cstate is a valid initial cstate *)
-        (exists init_chain init_ctx init_setup, 
-        init C init_chain init_ctx init_setup = Ok init_cstate) /\
-        (* with a trace to cstate *)
-        inhabited (ContractTrace C init_cstate cstate).
+Definition cstate_reachable (C : Contract Setup Msg State Error) (cstate : State) : Prop := 
+    exists init_cstate,
+    (* init_cstate is a valid initial cstate *)
+    (exists init_chain init_ctx init_setup, 
+    init C init_chain init_ctx init_setup = Ok init_cstate) /\
+    (* with a trace to cstate *)
+    inhabited (ContractTrace C init_cstate cstate).
 
-    Lemma inhab_trace_trans (C : Contract Setup Msg State Error) : 
-    forall from mid to, 
-        (ContractStep C mid to) -> 
-        inhabited (ContractTrace C from mid) -> 
-        inhabited (ContractTrace C from to).
-    Proof.
-        intros from mid to step.
-        apply inhabited_covariant.
-        intro mid_t.
-        apply (snoc mid_t step).
-    Qed.
+Lemma inhab_trace_trans (C : Contract Setup Msg State Error) : 
+forall from mid to, 
+    (ContractStep C mid to) -> 
+    inhabited (ContractTrace C from mid) -> 
+    inhabited (ContractTrace C from to).
+Proof.
+    intros from mid to step.
+    apply inhabited_covariant.
+    intro mid_t.
+    apply (snoc mid_t step).
+Qed.
 
 End ContractTrace.
 
 
-Context { Setup Setup' Msg Msg' State State' Error Error' : Type }
-    `{Serializable Msg}  `{Serializable Setup}  `{Serializable State}  `{Serializable Error}
-    `{Serializable Msg'} `{Serializable Setup'} `{Serializable State'} `{Serializable Error'}
-    {C : Contract Setup Msg State Error} {C' : Contract Setup' Msg' State' Error'}.
+Context `{Serializable Msg1} `{Serializable Setup1} `{Serializable State1} `{Serializable Error1}
+        `{Serializable Msg2} `{Serializable Setup2} `{Serializable State2} `{Serializable Error2}
+        {C1 : Contract Setup1 Msg1 State1 Error1} 
+        {C2 : Contract Setup2 Msg2 State2 Error2}.
+
 
 (* A theorem to use if we are inducting on C *)
 (* - the relationship always exists with some parallel C' 
         - rounding down/Uranium example. *)
 
 
-
 (** TODO a notion of it *corresponding* *)
 (* f : C -> C' *)
 Theorem left_cm_induction : 
     (* forall simple morphism and reachable bstate, *)
-    forall (f : simple_cm C C') bstate caddr (trace : ChainTrace empty_state bstate),
+    forall (f : ContractMorphism C1 C2) bstate caddr (trace : ChainTrace empty_state bstate),
     (* where C is at caddr with state cstate, *)
-    env_contracts bstate caddr = Some (C : WeakContract) -> 
-    exists (cstate : State), 
-    contract_state bstate caddr = Some cstate /\
-    (* every reachable cstate of C corresponds to a contract-reachable cstate' of C' ... *)
-    (exists (cstate' : State'),
-    (* 1. init_cstate' is a valid initial cstate of C'  *)
-    cstate_reachable C' cstate' /\
+    env_contracts bstate caddr = Some (C1 : WeakContract) -> 
+    exists (cstate1 : State1), 
+    contract_state bstate caddr = Some cstate1 /\
+    (* every reachable cstate1 of C1 corresponds to a contract-reachable cstate2 of C2 ... *)
+    (exists (cstate2 : State2),
+    (* 1. init_cstate2 is a valid initial cstate of C'  *)
+    cstate_reachable C2 cstate2 /\
     (* 2. cstate and cstate' are related by state_morph. *)
-    cstate' = state_morph C C' f cstate).
+    cstate2 = state_morph C1 C2 f cstate1).
 Proof.
-    intros f_simple * c_at_caddr.
-    destruct f_simple as [msg_morph setup_morph state_morph error_morph init_coherence recv_coherence].
+    intros f * c_at_caddr.
+    destruct f as [msg_morph setup_morph state_morph error_morph init_coherence recv_coherence].
     set (f := {|
         msg_morph := msg_morph;
         setup_morph := setup_morph;
@@ -984,7 +488,7 @@ Proof.
             exact clnil. }
         exists chain, ctx, (setup_morph setup).
         rewrite <- (init_coherence chain ctx setup).
-        destruct (init C chain ctx setup); 
+        destruct (init C1 chain ctx setup); 
         now try inversion init_some.
     (* non-recursive call *)
     -   intros.
@@ -999,18 +503,18 @@ Proof.
         exists (init_state').
         split.
         +   now exists init_c, init_ctx, init_s.
-        +   assert (ContractStep C' cstate_prev' (state_morph new_state))
+        +   assert (ContractStep C2 cstate_prev' (state_morph new_state))
                 as cstep.
             {   set (seq_new_state := state_morph new_state).
                 set (seq_msg := option_map msg_morph msg).
-                apply (build_contract_step C' cstate_prev' seq_new_state chain ctx seq_msg new_acts).
+                apply (build_contract_step C2 cstate_prev' seq_new_state chain ctx seq_msg new_acts).
                 (* now apply coherence *)
                 rewrite cstate_rel.
                 unfold seq_msg.
                 rewrite <- (recv_coherence chain ctx prev_state msg).
-                destruct (receive C chain ctx prev_state msg) eqn:H_rec;
+                destruct (receive C1 chain ctx prev_state msg) eqn:H_rec;
                 now try inversion receive_some. }
-            apply (inhab_trace_trans C' init_state' cstate_prev' (state_morph new_state)); 
+            apply (inhab_trace_trans C2 init_state' cstate_prev' (state_morph new_state)); 
             auto.
     (* recursive call *)
     -   intros.
@@ -1025,18 +529,18 @@ Proof.
         exists (init_state').
         split.
         +   now exists init_c, init_ctx, init_s.
-        +   assert (ContractStep C' cstate_prev' (state_morph new_state))
+        +   assert (ContractStep C2 cstate_prev' (state_morph new_state))
                 as cstep.
             {   set (seq_new_state := state_morph new_state).
                 set (seq_msg := option_map msg_morph msg).
-                apply (build_contract_step C' cstate_prev' seq_new_state chain ctx seq_msg new_acts).
+                apply (build_contract_step C2 cstate_prev' seq_new_state chain ctx seq_msg new_acts).
                 (* now apply coherence *)
                 rewrite cstate_rel.
                 unfold seq_msg.
                 rewrite <- (recv_coherence chain ctx prev_state msg).
-                destruct (receive C chain ctx prev_state msg) eqn:H_rec;
+                destruct (receive C1 chain ctx prev_state msg) eqn:H_rec;
                 now try inversion receive_some. }
-            apply (inhab_trace_trans C' init_state' cstate_prev' (state_morph new_state)); 
+            apply (inhab_trace_trans C2 init_state' cstate_prev' (state_morph new_state)); 
             auto.
     (* solve facts *)
     -   intros.
@@ -1054,9 +558,9 @@ Qed.
 (** TODO a notion of grabbing an init? or do you just do that if you can? *)
 (* f : C -> C' *)
 Theorem right_cm_induction:
-    forall (from to : State) (f : simple_cm C C'),
-    ContractTrace C from to ->
-    ContractTrace C' (state_morph C C' f from) (state_morph C C' f to).
+    forall (from to : State1) (f : ContractMorphism C1 C2),
+    ContractTrace C1 from to ->
+    ContractTrace C2 (state_morph C1 C2 f from) (state_morph C1 C2 f to).
 Proof.
     intros * ctrace.
     destruct f as [msg_morph setup_morph state_morph error_morph init_coherence recv_coherence].
@@ -1071,15 +575,15 @@ Proof.
     cbn.
     induction ctrace.
     -   exact clnil.
-    -   assert (ContractStep C' (state_morph mid) (state_morph to))
+    -   assert (ContractStep C2 (state_morph mid) (state_morph to))
         as cstep.
         {   destruct l as [s_chain s_ctx s_msg s_new_acts s_recv].
             set (seq_msg := option_map msg_morph s_msg).
-            apply (build_contract_step C' (state_morph mid) (state_morph to) s_chain s_ctx seq_msg s_new_acts).
+            apply (build_contract_step C2 (state_morph mid) (state_morph to) s_chain s_ctx seq_msg s_new_acts).
             (* now apply coherence *)
             unfold seq_msg.
             rewrite <- (recv_coherence s_chain s_ctx mid s_msg).
-            destruct (receive C s_chain s_ctx mid s_msg) eqn:H_rec;
+            destruct (receive C1 s_chain s_ctx mid s_msg) eqn:H_rec;
             now try inversion s_recv. }
         apply (snoc IHctrace cstep).
 Qed.
@@ -1091,6 +595,60 @@ Qed.
 
 End MorphismInduction.
 
+
+(** Equivalences of Contracts : an equivalence on just reachable states *)
+Section ContractEquiv.
+Context `{Serializable Msg1} `{Serializable Setup1} `{Serializable State1} `{Serializable Error1}
+        `{Serializable Msg2} `{Serializable Setup2} `{Serializable State2} `{Serializable Error2}.
+
+(* *)
+Record ContractTraceMorphism 
+    (C1 : Contract Setup1 Msg1 State1 Error1)
+    (C2 : Contract Setup2 Msg2 State2 Error2) := 
+    build_ct_morph {
+        (* a function *)
+        ct_state_morph : State1 -> State2 ;
+        (* TODO init -> init *)
+        (* coherence *)
+        cstep_morph : forall state1 state2,
+            cstate_reachable C1 state1 ->
+            ContractStep C1 state1 state2 ->
+            ContractStep C2 (ct_state_morph state1) (ct_state_morph state2) ;
+}.
+
+(* Identity *)
+(* Equality *)
+(* Composition *)
+
+Record ContractTraceIsomorphism
+    (C1 : Contract Setup1 Msg1 State1 Error1)
+    (C2 : Contract Setup2 Msg2 State2 Error2) := {
+    (* todo *)
+    }.
+
+Context {C1 : Contract Setup1 Msg1 State1 Error1} 
+        {C2 : Contract Setup2 Msg2 State2 Error2}.
+
+(** Weak Equivalence : an equivalence on reachable states *)
+Definition is_equivalence (f : ContractMorphism C1 C2) (g : ContractMorphism C2 C1) : Prop := 
+    is_iso (msg_morph   C1 C2 f) (msg_morph   C2 C1 g) /\
+    is_iso (setup_morph C1 C2 f) (setup_morph C2 C1 g) /\
+    forall cstate1 cstate2,
+    (* f and g are isomorphic on reachable states *)
+    (cstate_reachable C1 cstate1 -> compose (state_morph C2 C1 g) (state_morph C1 C2 f) cstate1 = cstate1) /\
+    (cstate_reachable C2 cstate2 -> compose (state_morph C1 C2 f) (state_morph C2 C1 g) cstate2 = cstate2).
+
+(** Isomorphism -> Equivalence *)
+Proposition iso_to_equiv_cm (f : ContractMorphism C1 C2) (g : ContractMorphism C2 C1) : 
+    is_iso_cm f g -> is_equivalence f g.
+Admitted.
+
+(** equivalence -> contract trace equivalence *)
+Proposition equiv_to_ctmorph (f : ContractMorphism C1 C2) (g : ContractMorphism C2 C1) :
+    is_equivalence f g -> ContractTraceIsomorphism C1 C2.
+Admitted.
+
+End ContractEquiv.
 
 
 End ContractMorphisms.
