execution/theories/ContractSystems.v
@@ -20,11 +20,10 @@ Definition pair_fun2 {S T S' T' S'' T'' : Type}
     let (s,t) := x in let (s', t') := y in (f s s', g t t').
 
 
-Context {Base : ChainBase}.
-
 (** We have some interesting categorical properties, including the existence of a terminal
-    contract. (Note that we have not yet proved uniqueness of the terminal morphism.) *)
+contract. (Note that we have not yet proved uniqueness of the terminal morphism.) 
 Section TerminalContract.
+Context {Base : ChainBase}.
 Import ListNotations.
 Set Nonrecursive Elimination Schemes.
 
@@ -139,10 +138,11 @@ Definition null_morphism : ContractMorphism C null_contract :=
 
 (* TODO: Prove uniqueness *)
 
-End TerminalContract.
+End TerminalContract. *)
 
 
 Section ContractTransformations.
+Context {Base : ChainBase}.
 
 (** We define the product of two contracts *)
 Section ContractProducts.
@@ -284,7 +284,6 @@ Definition sum_contract
 
 End ContractSums.
 
-
 Section ContractSumsCorrect.
 Context { Setup Setup' Setup'' Msg Msg' Msg'' State State' State'' Error Error' Error'' : Type }
     `{Serializable Msg} `{Serializable Setup} `{Serializable State} `{Serializable Error}
@@ -299,16 +298,17 @@ Lemma sum_contract_associative : contracts_isomorphic
         (sum_contract (sum_contract C C') C'').
 Proof. Admitted.
 
+(*
 Theorem sum_contract_projects_left : 
     exists (f : ContractMorphism (sum_contract C C') (sum_contract C null_contract)),
         is_surj_cm f.
-Proof. Admitted.
+Proof. Admitted. 
 
 Theorem sum_contract_projects_right : 
     exists (f : ContractMorphism (sum_contract C C') (sum_contract null_contract C')),
         is_surj_cm f.
 Proof. Admitted.
-
+*)
 Theorem sum_contract_embeds_left : 
     exists (f : ContractMorphism C (sum_contract C C')),
         is_inj_cm f.
@@ -440,375 +440,80 @@ End PointedContract.
 End ContractTransformations.
 
 
-(** There have been some examples of contracts which aren't iso (counter, counter *2 for eg)
-    but would be for all reachable states.
-    In that eg, counter *2 always has an even number in storage, so there is an isomorphism
-    ** OF REACHABLE STATES **.
-    That's different from a contract isomorphism. *)
 
 
 
+(** Notation for a system of contracts *)
+Section ContractSystem.
+
+(** On one single chain *)
+Definition CSys (B : ChainBase) : Type := list (@WeakContract B).
+(* plus contract preimages? *)
 
 
+(** Multi-chain *)
+Definition CSysS (B1 B2 : ChainBase) : Type := list (@WeakContract B1) * list (@WeakContract B2).
 
 
-
-
-(** TODO 
-
-Section MultiChainWeakEquivalences.
-
-Definition MultiChainState : Type := @ChainState Base1 * @ChainState Base2.
-Definition MultiChainStep (prev_multi_bstate : MultiChainState) (next_multi_bstate : MultiChainState) : Type := 
-        @ChainStep Base1 (fst prev_multi_bstate) (fst next_multi_bstate) +
-        @ChainStep Base2 (snd prev_multi_bstate) (snd next_multi_bstate) +
-       (@ChainStep Base1 (fst prev_multi_bstate) (fst next_multi_bstate) *
-        @ChainStep Base2 (snd prev_multi_bstate) (snd next_multi_bstate)).
-Definition MultiChainTrace := ChainedList MultiChainState MultiChainStep.
-
-(* multi-chain contract : Defn 6.3.2 *)
-
-
-(* multi-chain null contract *)
-
-(* multi-chain morphism *)
-Definition multichain_empty_state : MultiChainState := (empty_state, empty_state).
-
-Definition multichain_reachable (mstate : MultiChainState) : Prop := 
-    reachable (fst mstate) /\ reachable (snd mstate).
-
-(* A multi-chain morphism is a morphism of linked lists *)
-(* TODO restrict to reachability? *)
-Record MultiChainMorphism := build_multi_chain_morphism {
-    multichainstate_morph : MultiChainState -> MultiChainState ; 
-    multi_empty_fixpoint : 
-        multichainstate_morph multichain_empty_state = multichain_empty_state ; 
-    multichainstep_morph : 
-        forall mstate1 mstate2, 
-        MultiChainStep mstate1 mstate2 -> 
-        MultiChainStep (multichainstate_morph mstate1) (multichainstate_morph mstate2) ;
-}.
-
-(* Lemma : takes reachable states to reachable states *)
-(* TODO AFTER you sorted out contract morphisms *)
-
-(* composition of multi-chain morphisms *)
-(* an auxiliary lemma *)
-Lemma multichain_compose_fixpoint_result (mch1 mch2 : MultiChainMorphism) : 
-    compose (multichainstate_morph mch2) (multichainstate_morph mch1) multichain_empty_state =
-    multichain_empty_state.
-Proof. Admitted.
-
-(* composition of multi-chain morphisms *)
-Definition composition_mch (mch1 mch2 : MultiChainMorphism) : MultiChainMorphism := {| 
-    multichainstate_morph := 
-        compose (multichainstate_morph mch1) (multichainstate_morph mch2) ; 
-    multi_empty_fixpoint := multichain_compose_fixpoint_result mch2 mch1 ;
-    multichainstep_morph := (fun b1 b2 => 
-        compose 
-            (multichainstep_morph mch2 
-                (multichainstep_morph mch1 b1)
-                (multichainstep_morph mch2 b2))
-            (multichainstep_morph mch1 b1 b2)) ;
-|}.
-
-(* composition is associative *)
-Lemma composition_assoc_mch : forall mch1 mch2 mch3, 
-    composition_mch (composition_mch mch3 mch2) mch1 = 
-    composition_mch mch3 (composition_mch mch2 mch1).
-Proof. (* proof omitted *) Qed.
-
-(*** identity morphism *)
-(* an auxiliary lemma *)
-Lemma multi_empty_fixpoint_id : 
-    @id MultiChainState multichain_empty_state = multichain_empty_state.
-Proof. auto. Qed.
-
-(* the identity multi-chain morphism *)
-Definition id_mch : MultiChainMorphism := {| 
-    multichainstate_morph := @id MultiChainState ; 
-    multi_empty_fixpoint := multi_empty_fixpoint_id ;
-    multichainstep_morph := (fun b1 b2 => @id (MultiChainStep b1 b2)) ;
-|}.
-
-(* left and right composition results *)
-Lemma composition_mch_left : forall mch, composition_mch id_mch mch = mch.
-Proof. (* proof omitted *) Qed.
-
-Lemma composition_mch_right : forall mch, composition_mch mch id_mch = mch.
-Proof. (* proof omitted *) Qed.
-
-End MultiChainWeakEquivalences.
-
-
-
-Section WeakContractMorphisms.
-
-(* a weak morphism between a system of contracts and a monolithic contract *)
-
-
-(* THEN one corresponding to each of these constructions ^^ (with conditions on what's needed, e.g. account balances unchanged) *)
-
-End WeakContractMorphisms.
-
-
-Section ChainMorphisms.
-
-Record ChainMorphism := build_chain_morphism {
-    chainstate_morph : ChainState -> ChainState ; 
-    chainstep_morph : 
-        forall bstate1 bstate2, 
-        ChainStep bstate1 bstate2 -> 
-        ChainStep (chainstate_morph bstate1) (chainstate_morph bstate2) ;
-}.
-
-(* the identity chain morphism *)
-Definition id_chm : ChainMorphism := {| 
-    chainstate_morph := id_fun ChainState ; 
-    chainstep_morph := (fun b1 b2 => id_fun (ChainStep b1 b2)) ; |}.
-
-Definition composition_chm (chm2 chm1 : ChainMorphism) : ChainMorphism := {| 
-    chainstate_morph := compose (chainstate_morph chm2) (chainstate_morph chm1) ;
-    chainstep_morph  := (fun b1 b2 => 
-        compose 
-            (chainstep_morph chm2 
-                (chainstate_morph chm1 b1) 
-                (chainstate_morph chm1 b2)) 
-            (chainstep_morph chm1 b1 b2)) ;
-|}.
-
-Lemma composition_chm_left : forall chm, composition_chm id_chm chm = chm.
-Proof. 
-    intro. unfold composition_chm. 
-    destruct chm. f_equal; simpl.
-Qed.
-
-Lemma composition_chm_right : forall chm, composition_chm chm id_chm = chm.
-Proof. 
-    intro. unfold composition_chm. 
-    destruct chm. f_equal; simpl.
-Qed.
-
-Lemma composition_assoc_chm : forall chm1 chm2 chm3, 
-    composition_chm (composition_chm chm3 chm2) chm1 = 
-    composition_chm chm3 (composition_chm chm2 chm1).
-Proof.
-    intros. unfold composition_chm. f_equal.
-Qed.
-
-(* chain isomoprhisms, which are bisimulations of blockchains *)
-Definition is_iso_chm (f g : ChainMorphism) : Prop := 
-    composition_chm g f = id_chm /\ 
-    composition_chm f g = id_chm.
-
-End ChainMorphisms.
-
-(*  Some conditions under which a system of contracts can be 
-    contracted via a chain (e.g. bisimulated) *)
-
-Section SystemContraction.
-Import ListNotations.
-
-Definition cm_lift' 
-    { Setup Setup' Msg Msg' State State' Error Error' : Type }
-    `{Serializable Msg}  `{Serializable Setup}  `{Serializable State}  `{Serializable Error}
-    `{Serializable Msg'} `{Serializable Setup'} `{Serializable State'} `{Serializable Error'}
-    {C : Contract Setup Msg State Error} {C' : Contract Setup' Msg' State' Error'} : 
-    (f : ContractMorphism C C') -> ChainMorphism.
-
-
-(* the chainstate (cst) morphism : system to monolithic *)
-Definition cst_system_to_mono 
-    { Setup Setup' Msg Msg' State State' Error Error' : Type }
-    `{Serializable Msg}  `{Serializable Setup}  `{Serializable State}  `{Serializable Error}
-    `{Serializable Msg'} `{Serializable Setup'} `{Serializable State'} `{Serializable Error'}
-    {C : Contract Setup Msg State Error} {C' : Contract Setup' Msg' State' Error'}
-    (caddr1 caddr2 : Address)
-    (bstate : ChainState) : ChainState := 
-    {| chain_state_env :=
-       {| env_chain :=
-            {| chain_height := 0;
-               current_slot := 0;
-               finalized_height := 0; |};
-          env_account_balances a := 0%Z;
-          env_contract_states a := None;
-          env_contracts a := None; |};
-     chain_state_queue := [] |}.
-
-(* the chainstep (csp) morphism : system to monolithic *)
-Definition csp_system_to_mono
-
-(* the chain morphism (chm) : system to monolithic *)
-Definition chm_system_to_mono 
-
-
-
-
-
-Definition chm_mono_to_system
-
-
-Theorem system_contraction 
-        { Setup Setup' Msg Msg' State State' Error Error' : Type }
-        `{Serializable Msg}  `{Serializable Setup}  `{Serializable State}  `{Serializable Error}
-        `{Serializable Msg'} `{Serializable Setup'} `{Serializable State'} `{Serializable Error'}
-        {C : Contract Setup Msg State Error} {C' : Contract Setup' Msg' State' Error'} : 
-    forall bstate caddr1 caddr2, 
-    (* such that caddr1 is C and caddr2 is C' *)
-
-    (* the chain morphism defined above *)
-
-
-End SystemContraction.
-
-
-(** A weak equivalence of Environments and ChainStates *)
-Section ChainStateWeakEquivalence.
-(* SETTING:
-    - I have a system of contracts, which consists of: 
-        - a POINTED set of addresses, which is the point of contraction (perhaps define this yourself)
-    - I need to transform it into a disjoint sum of contracts living at one address
-    - And then prove a bisimulation
+(** Systems should have an interface:
+    - a (collective) message type 
+    - collective storage 
+    - collective balance (this might be tricky ...)
+    - a collective trace
 *)
 
-Definition ActionWeakTransform (* 
-  - transforms actions into the contracts in the system into actions into the joined contract 
-  - this changes:
-    - from (modular => monolithic)
-    - to (modular => monolithic)
-    - msg (msg => inl msg or inr msg, etc) -- perhaps you define this when you define the contraction
-  - TODO what to do about deployments?
-*)
-
-Definition EnvironmentWeakEquiv (e1 e2 : Environment) 
-    (mon : (Address * WeakContract)) (* the monolithic contract *)
-    (sys : list (Address * WeakContract)) (* the system of contracts*) := 
-    build_env_weak_eq {
-        chain_weak_eq : 
-        (* we need to adjust chain height to account for deployments and, later, *) ;
-        account_balances_weak_eq : 
-            forall a,
-                (* if a not in list *)
-                (* then same *)
-                (* otherwise, sum of the list balances = the monolithic balance *) ;
-        contracts_weak_eq : 
-            forall a,
-                (* if a not in list *)
-                (* then same *)
-                (* otherwise, None in list, mon at mon_addr *) ;
-        contract_states_weak_eq : 
-            forall a,
-            (* if a not in list *)
-            (* then same *)
-            (* otherwise, None in list, mon's state at mon_addr *) ;
-    }.
-
-(*
-  - Chain : ?
-  - Balances : sum of balance of system should always equal balance of 
-  - (weak) Contracts : monolithic address has monolithic contract; each 
-  - States : states are none at old addresses, are the combined state at the pointed address 
-*)
+End ContractSystem.
 
 
-Definition ChainStateWeakEquiv (* 
-  - list Action : ?
-*)
+(** Morphisms of Systems of Contracts *)
+Section SystemMorphism.
 
 
-(*
-  - this is a NOTION of equivalence, parameterized over a system of contracts.
-  - you need to prove that this notion of equivalence is actually a BISIMULATION
-  - then provide sufficient conditions to achieve this ...
-     - the idea being that you take a system and combine it in any way listed above ^^.
-       then you have a single contract you can reason about.
-*)
+End SystemMorphism.
 
 
+(** Equivalences of Systems of Contracts *)
+Section SysEquiv.
 
-Context 
-    (* we can lift a morphism of contracts, parameterized by the morphpism f and the address of C1 *)
-    { Setup Setup' Msg Msg' State State' Error Error' : Type }
-    `{Serializable Msg}  `{Serializable Setup}  `{Serializable State}  `{Serializable Error}
-    `{Serializable Msg'} `{Serializable Setup'} `{Serializable State'} `{Serializable Error'}
-    {C1 : Contract Setup Msg State Error} {C2 : Contract Setup' Msg' State' Error'}
-    {f : ContractMorphism C1 C2}.
+(* first strong equiv *)
 
-Definition wc_dec_eq : forall w1 w2 : WeakContract, {w1 = w2} + {w1 <> w1} := todo "".
-Declare Scope wc_scope.
-Delimit Scope wc_scope with wc.
-Bind Scope wc_scope with WeakContract.
-Infix "=?" := wc_dec_eq (at level 70) : wc_scope.
-
-(* Given f, we can transform actions *)
-Definition action_transform { addrs : set Address } (native_env : Environment) (a : Action) : Action := {| 
-    act_origin := act_origin a ;
-    act_from := act_from a ;
-    act_body := 
-        match act_body a with 
-        (* contract calls into C1 change to calls into C2 *)
-        | act_call to amt msg => 
-            match env_contracts native_env to with 
-            | Some wc => 
-                if (wc =? contract_to_weak_contract C1)%wc
-                then act_call to amt msg
-                else act_body a
-            | None => act_body a
-            end
-        (* we deploy C2 instead of C1 *)
-        | act_deploy amt c setup => 
-            if (c =? contract_to_weak_contract C1)%wc
-            then act_deploy amt (contract_to_weak_contract C2) setup
-            else act_body a
-        (* all amounts stay the same, so we do not change transfers *)
-        | act_transfer _ _ => act_body a 
-        end
-|}.
-
-(* A morphism of Environments, parameterized implicitly over f by swapping out C2 for C1 *)
-Record EnvironmentMorphism (e1 e2 : Environment) := 
-    build_env_morphism {
-        chain_eq' : env_chain e1 = env_chain e2 ;
-        account_balances_eq' :
-            forall a, env_account_balances e1 a = env_account_balances e2 a ;
-        contracts_morph :
-            forall a, 
-                env_contracts e2 a = 
-                match env_contracts e1 a with 
-                | Some wc => 
-                    if (wc =? contract_to_weak_contract C1)%wc 
-                    then Some (contract_to_weak_contract C2) 
-                    else Some wc
-                | None => None 
-                end ;
-        contract_states_morph : 
-            forall a, 
-                env_contract_states e2 a = 
-                match env_contracts e1 a with 
-                | Some wc => 
-                    if (wc =? contract_to_weak_contract C1)%wc 
-                    then (option_fun (serialize_function state_morph)) (env_contract_states e1 a)
-                    else env_contract_states e1 a
-                | None => env_contract_states e1 a
-                end ;
-}.
-
-(* A morphism of ChainStates, parameterized implicitly over f *)
-Record ChainStateMorphism (cstate1 cstate2 : ChainState) := 
-    build_chainstate_morphism {
-        env_morph   : EnvironmentMorphism cstate1 cstate2 ;
-        queue_morph : chain_state_queue cstate2 = 
-                      List.map (action_transform cstate1) (chain_state_queue cstate1) ;
-    }.
-
-End ChainStateWeakEquivalence.
-
-
-Section WeakContractMorphismLift.
-
-
-
-End WeakContractMorphismLift.
-
+(** Some notion of **shared trace** 
+    - their balances 
+    - their states 
+    - incoming/outgoing messages 
 
 *)
+
+(** Weak equivalences (just reachable) *)
+
+End SysEquiv.
+
+
+
+(** Multi-chain Contracts and Systems of Multi-chain Contracts *)
+Section MultiChainContract.
+Context {B1 B2: ChainBase}
+    { Setup1 Setup2 Msg1 Msg2 State1 State2 Error1 Error2 : Type }
+    `{m1_ser : Serializable Msg1} `{s1_ser : Serializable Setup1} 
+    `{st1_ser : Serializable State1} `{er1_ser : Serializable Error1}
+    `{m2_ser : Serializable Msg2} `{s2_ser : Serializable Setup2} 
+    `{st2_ser : Serializable State2} `{er2_ser : Serializable Error2}.
+
+(* A multi-chain contract *)
+Definition MContract : Type := 
+    (@Contract B1 Setup1 Msg1 State1 Error1 s1_ser m1_ser st1_ser er1_ser + 
+     @Contract B2 Setup2 Msg2 State2 Error2 s2_ser m2_ser st2_ser er2_ser)%type.
+
+
+(* A system of multi-chain contracts *)
+
+
+(* Equivalence (both strong and weak) of multi-chain contracts *)
+
+
+
+(* should all be a straightforward generalization of what's above *)
+
+
+
+End MultiChainContract.
